feat: `debug` option to run validation on `AxEffect` state
Also, using this option, I've added a more minimal failing test case to showcase the memory bug

Tests/Tactics/Sym.lean
@@ -5,6 +5,8 @@ Author(s): Alex Keizer
 -/
 import Proofs.«AES-GCM».GCMGmultV8Sym
 
+set_option Tactic.sym.debug true
+
 namespace GCMGmultV8Program
 
 -- Test the behaviour of `sym_n` when `h_err` and `h_sp` are not present
@@ -19,3 +21,27 @@ namespace GCMGmultV8Program
   · sorry
   · exact (sorry : read_err s0 = .None)
   done
+
+
+namespace SimpleMemory
+
+def program := def_program [
+    (0x4005b8#64 , 0xb9000fe0#32), -- str w0, [sp, #12]
+  ]
+
+#genStepEqTheorems program
+
+example
+    (sf s0 : ArmState)
+    (h_program : s0.program = program)
+    (h_run : sf = run 1 s0)
+    (h_err : read_err s0 = .None)
+    (h_pc : read_pc s0 = 0x4005b8#64)
+    (h_sp : CheckSPAlignment s0)
+    (h_s0_x0 : r (.GPR 0#5) s0 = x)
+    (h_s0_x31 : r (.GPR 31#5) s0 = y) :
+    read_mem_bytes 4 (y + 12#64) s0 = (x.zeroExtend 32) := by
+  sym_n 1
+  sorry
+
+end SimpleMemory
