Tactics/Sym.lean
@@ -240,7 +240,10 @@ def explodeStep (c : SymContext) (hStep : Expr) : TacticM Unit :=
                 #[eff.currentState, spEff.value, spEff.proof, hAligned]
             pure { eff with stackAlignmentProof? }
 
-    withMainContext <|
+    withMainContext <| do
+      if ←(getBoolOption `Tactic.sym.debug) then
+        eff.validate
+
       eff.addHypothesesToLContext s!"h_{c.next_state}_"
 
 /-- A tactic wrapper around `explodeStep`.
